Serialize integers

examples/lowparse/LowParse.Impl.Int.fst
@@ -85,3 +85,144 @@ let parse_u32_st_nochk :
 inline_for_extraction
 let parse_u32_st : parser_st (parse_u32) =
   parse_total_constant_size 4ul parse_u32_st_nochk
+
+module HST = FStar.HyperStack.ST
+module B = FStar.Buffer
+
+inline_for_extraction
+val serialize_u8
+  (i: U8.t)
+  (dest: S.bslice)
+: HST.Stack (S.bslice * S.bslice)
+  (requires (fun h ->
+    U32.v (S.length dest) >= 1 /\
+    S.live h dest
+  ))
+  (ensures (fun h (destl, destr) h' ->
+    S.is_concat dest destl destr /\
+    S.length destl == 1ul /\
+    S.live h' destr /\
+    B.modifies_1 (S.as_buffer destl) h h' /\
+    exactly_parses h' parse_u8 destl (fun v ->
+    v == i
+  )))
+
+#set-options "--z3rlimit 64"
+
+let serialize_u8 i dest =
+  let destl = S.truncate_slice dest 1ul in
+  let b = S.as_buffer destl in
+  B.upd b 0ul i;
+  let destr = S.advance_slice dest 1ul in
+  (destl, destr)
+
+#reset-options
+
+module Cast = FStar.Int.Cast
+
+inline_for_extraction
+val serialize_u16
+  (i: U16.t)
+  (dest: S.bslice)
+: HST.Stack (S.bslice * S.bslice)
+  (requires (fun h ->
+    U32.v (S.length dest) >= 2 /\
+    S.live h dest
+  ))
+  (ensures (fun h (destl, destr) h' ->
+    S.is_concat dest destl destr /\
+    S.length destl == 2ul /\
+    S.live h' destr /\
+    B.modifies_1 (S.as_buffer destl) h h' /\
+    exactly_parses h' parse_u16 destl (fun v ->
+    v == i
+  )))
+
+#set-options "--z3rlimit 64 --max_fuel 8 --max_ifuel 8"
+
+let serialize_u16 i dest =
+  let destl = S.truncate_slice dest 2ul in
+  let b = S.as_buffer destl in
+  let v256 = U16.uint_to_t 256 in
+  B.upd b 1ul (Cast.uint16_to_uint8 (U16.rem i v256));
+  B.upd b 0ul (Cast.uint16_to_uint8 (U16.div i v256));
+  let destr = S.advance_slice dest 2ul in
+  let h' = HST.get () in
+  assert (Seq.equal (S.as_seq h' destl) (E.n_to_be 2ul (U16.v i)));
+  Seq.lemma_eq_elim (S.as_seq h' destl) (E.n_to_be 2ul (U16.v i));
+  assert (E.be_to_n (S.as_seq h' destl) == U16.v i);
+  (destl, destr)
+
+#reset-options
+
+val serialize_u32_aux
+  (i: U32.t)
+  (s: bytes32)
+: Ghost bytes32
+  (requires (Seq.length s == 4))
+  (ensures (fun s' ->
+    Seq.length s' == 4 /\
+    Seq.equal s' (E.n_to_be 4ul (U32.v i))
+  ))
+
+#set-options "--z3rlimit 128 --max_fuel 8 --max_ifuel 8"
+
+let serialize_u32_aux i s =
+  let v256 = U32.uint_to_t 256 in
+  let j3 = Cast.uint32_to_uint8 (U32.rem i v256) in
+  let s3 = Seq.upd s 3 j3 in
+  let i2 = U32.div i v256 in
+  let j2 = Cast.uint32_to_uint8 (U32.rem i2 v256) in
+  let s2 = Seq.upd s3 2 j2 in
+  let i1 = U32.div i2 v256 in
+  let j1 = Cast.uint32_to_uint8 (U32.rem i1 v256) in
+  let s1 = Seq.upd s2 1 j1 in
+  let j0 = Cast.uint32_to_uint8 (U32.div i1 v256) in
+  Seq.upd s1 0 j0
+
+#reset-options
+
+inline_for_extraction
+val serialize_u32
+  (i: U32.t)
+  (dest: S.bslice)
+: HST.Stack (S.bslice * S.bslice)
+  (requires (fun h ->
+    U32.v (S.length dest) >= 4 /\
+    S.live h dest
+  ))
+  (ensures (fun h (destl, destr) h' ->
+    S.is_concat dest destl destr /\
+    S.length destl == 4ul /\
+    S.live h' destr /\
+    B.modifies_1 (S.as_buffer destl) h h' /\
+    exactly_parses h' parse_u32 destl (fun v ->
+    v == i
+  )))
+
+#set-options "--z3rlimit 64"
+
+let serialize_u32 i dest =
+  let destl = S.truncate_slice dest 4ul in
+  let b = S.as_buffer destl in
+  let h = HST.get () in
+  let v256 = U32.uint_to_t 256 in
+  let j3 = Cast.uint32_to_uint8 (U32.rem i v256) in
+  B.upd b 3ul j3;
+  let i2 = U32.div i v256 in
+  let j2 = Cast.uint32_to_uint8 (U32.rem i2 v256) in
+  B.upd b 2ul j2;
+  let i1 = U32.div i2 v256 in
+  let j1 = Cast.uint32_to_uint8 (U32.rem i1 v256) in
+  B.upd b 1ul j1;
+  let j0 = Cast.uint32_to_uint8 (U32.div i1 v256) in
+  B.upd b 0ul j0;
+  let destr = S.advance_slice dest 4ul in
+  let h' = HST.get () in
+  assert (S.as_seq h' destl == serialize_u32_aux i (S.as_seq h destl));
+  assert (Seq.equal (S.as_seq h' destl) (E.n_to_be 4ul (U32.v i)));
+  Seq.lemma_eq_elim (S.as_seq h' destl) (E.n_to_be 4ul (U32.v i));
+  assert (E.be_to_n (S.as_seq h' destl) == U32.v i);
+  (destl, destr)
+
+#reset-options
